Instantiate hash functions

Extraction/src/Core.ml
@@ -1,0 +1,26 @@
+(* Don't import this file directly! Use the implementations provided by Impl.ml *)
+
+open TypesImpl.TypesImpl
+
+let clist_to_string cl = String.concat "" (List.map (String.make 1) cl)
+let string_to_clist s = List.init (String.length s) (String.get s)
+
+(* Implemented here and extracted into Impl.ml *)
+let hash_of_tx (tx_cl : char list) =
+  let s = clist_to_string tx_cl in
+  let hash_str =
+    "0x" ^ Cryptokit.transform_string (Cryptokit.Hexa.encode ())
+     (Cryptokit.hash_string (Cryptokit.Hash.sha256 ()) s) in
+  let hash_cl = string_to_clist hash_str in
+  hash_cl
+
+let hash_of_block (b : coq_Block) =
+  let fmt = format_of_string "%s|%s" in
+  let s = Printf.sprintf fmt
+    (clist_to_string b.prevBlockHash)
+    (String.concat "&" (List.map clist_to_string b.txs)) in
+  let hash_str =
+    "0x" ^ Cryptokit.transform_string (Cryptokit.Hexa.encode ())
+      (Cryptokit.hash_string (Cryptokit.Hash.sha256 ()) s) in
+  let hash_cl = string_to_clist hash_str in
+  hash_cl
