Extraction/src/Util.ml
@@ -1,6 +1,6 @@
 open Forests
 
-module Types = Impl.TypesImpl
+module Types = TypesImpl.TypesImpl
 module ConsensusParams = Impl.ProofOfWork
 module ForestImpl = Forests (Types) (ConsensusParams)
 
@@ -13,8 +13,9 @@ let string_of_tx tx = clist_to_string tx
 let string_of_hash h = clist_to_string h
 
 let string_of_block (b : coq_Block) =
-  let fmt = format_of_string "{prev = %s, txs = %s}" in
+  let fmt = format_of_string "%s = {prev = %s, txs = %s}" in
   Printf.sprintf fmt
+    (string_of_hash (ConsensusParams.hashB b))
     (string_of_hash b.prevBlockHash)
     (String.concat " " (List.map string_of_tx b.txs))
 
