Extraction/Impl.v
@@ -3,7 +3,7 @@ Require Import ssreflect ssrbool ssrnat eqtype ssrfun seq fintype path.
 From fcsl
 Require Import ordtype unionmap.
 From Toychain
-Require Import Types Parameters Address.
+Require Import Types TypesImpl Parameters Address.
 Require Import BinNat BinNatDef.
 Require Import HexString String Ascii.
 Set Implicit Arguments.
@@ -11,242 +11,14 @@ Unset Strict Implicit.
 Unset Printing Implicit Defensive.
 
 (* TODO: find a way to remove this stuff from the extraction! *)
-Section NEq.
-Lemma eq_NP : Equality.axiom N.eqb.
-Proof.
-case=>[x|p x]//=; case: x.
-by constructor 1; apply N.Private_Tac.eq_refl.
-by constructor 2.
-by constructor 2.
-move=>p'; case X: (BinPos.Pos.eqb p p').
-by constructor 1; move/BinPos.Peqb_true_eq: X=>->.
-by constructor 2; case; move/BinPos.Pos.eqb_neq: X.
-Qed.
-End NEq.
-
-
-Section NOrd.
-Lemma irr_ltbN : irreflexive N.ltb.
-Proof. by case=>[|n]//; apply N.ltb_irrefl. Qed.
-
-Lemma trans_ltbN : transitive N.ltb.
-Proof.
-by move=>x y z; move=>/N.ltb_lt A /N.ltb_lt B;
-   apply/N.ltb_lt; move: (N.lt_trans _ _ _ A B).
-Qed.
-
-Lemma total_ltbN x y : [|| N.ltb x y, x == y | N.ltb y x].
-Proof.
-apply/or3P; case: (N.compare_spec x y).
-by move=>->; constructor 2.
-by constructor 1; apply/N.ltb_lt.
-by constructor 3; apply/N.ltb_lt.
-Qed.
-
-Definition N_ordMixin := Eval hnf in OrdMixin irr_ltbN trans_ltbN total_ltbN.
-Canonical N_ordType := Eval hnf in OrdType N N_ordMixin.
-End NOrd.
-
-Section StringEq.
-
-(* Define so we can reuse proofs from above *)
-Definition ascii_eqb (a b : ascii) : bool :=
- match a, b with
- | Ascii a0 a1 a2 a3 a4 a5 a6 a7,
-   Ascii b0 b1 b2 b3 b4 b5 b6 b7 =>
-   (a0 == b0) && (a1 == b1) && (a2 == b2) && (a3 == b3)
-   && (a4 == b4) && (a5 == b5) && (a6 == b6) && (a7 == b7)
- end.
-
-Lemma ascii_eqP : Equality.axiom ascii_eqb.
-Proof.
-case=>a0 a1 a2 a3 a4 a5 a6 a7; case=>b0 b1 b2 b3 b4 b5 b6 b7.
-rewrite/ascii_eqb.
-(case:a0;case:b0=>/=; do? by constructor);
-(case:a1;case:b1=>/=; do? by constructor);
-(case:a2;case:b2=>/=; do? by constructor);
-(case:a3;case:b3=>/=; do? by constructor);
-(case:a4;case:b4=>/=; do? by constructor);
-(case:a5;case:b5=>/=; do? by constructor);
-(case:a6;case:b6=>/=; do? by constructor);
-(case:a7;case:b7=>/=; do? by constructor).
-Qed.
-
-Definition ascii_eqMixin := EqMixin ascii_eqP.
-Canonical ascii_eqType := Eval hnf in EqType ascii ascii_eqMixin.
-
-Fixpoint string_eqb (s1 s2 : string): bool :=
- match s1, s2 with
- | EmptyString, EmptyString => true
- | String c1 s1', String c2 s2' => ascii_eqb c1 c2 && string_eqb s1' s2'
- | _,_ => false
-end.
-
-Lemma ascii_eqb_refl x : ascii_eqb x x.
-Proof. by case: x=>b0 b1 b2 b3 b4 b5 b6 b7//=; rewrite !eq_refl. Qed.
-
-Lemma string_eqP : Equality.axiom string_eqb.
-Proof.
-rewrite/Equality.axiom=>s1; elim: s1; first by case; constructor.
-move=>x xs Hi; case; first by constructor.
-move=>y ys; case E: (x == y).
-- move/eqP in E; rewrite -E//=.
-  rewrite ascii_eqb_refl//=; move: (Hi ys).
-  case; first by move=>->; constructor.
-  by move=>X; constructor; case.
-move/eqP in E; have X: (String x xs <> String y ys) by case.
-specialize (Hi ys); rewrite/string_eqb.
-case Q: (ascii_eqb x y)=>//=.
-by move: (ascii_eqP x y Q).
-by constructor.
-Qed.
-
-Definition string_eqMixin := EqMixin string_eqP.
-Canonical string_eqType := Eval hnf in EqType string string_eqMixin.
-End StringEq.
-
-Section StringOrd.
-
-Lemma ascii_eqb_N x y :
-  ascii_eqb x y = (N_of_ascii x == N_of_ascii y).
-Proof.
-case E: (x == y); first by move/eqP: E=>->; rewrite ascii_eqb_refl eq_refl.
-have X: (ssrfun.cancel N_of_ascii ascii_of_N)
-  by move=>z; apply ascii_N_embedding.
-move: (can_eq X x y)=>->; rewrite E.
-case Z: (ascii_eqb x y)=>//.
-by move: (ascii_eqP x y Z); move/eqP: E.
-Qed.
-
-Definition ascii_ltb (a b : ascii) : bool := N.ltb (N_of_ascii a) (N_of_ascii b).
-
-Lemma irr_ascii : irreflexive ascii_ltb.
-by rewrite/irreflexive/ascii_ltb=>x; apply irr_ltbN.
-Qed.
-
-Lemma trans_ascii : transitive ascii_ltb.
-by rewrite/transitive/ascii_ltb=>x y z; apply trans_ltbN.
-Qed.
-
-Lemma total_ascii x y : [|| ascii_ltb x y, x == y | ascii_ltb y x].
-Proof.
-rewrite/ascii_ltb.
-suff X: ((x == y) = (N_of_ascii x == N_of_ascii y))
-  by rewrite X; apply total_ltbN.
-case Q: (x == y); first by move/eqP: Q=>->; rewrite eq_refl.
-rewrite -ascii_eqb_N; case X: (ascii_eqb x y)=>//=.
-by move: (ascii_eqP x y X); move/eqP: Q.
-Qed.
-
-Definition ascii_ordMixin := OrdMixin irr_ascii trans_ascii total_ascii.
-Canonical Structure ascii_ordType := Eval hnf in OrdType ascii ascii_ordMixin.
-
-Fixpoint string_ltb (s1 s2 : string): bool :=
- match s1, s2 with
- | EmptyString, EmptyString => false
- | EmptyString, _ => true
- | _, EmptyString => false
- | String c1 s1', String c2 s2' => ascii_ltb c1 c2 || (ascii_eqb c1 c2 && string_ltb s1' s2')
-end.
-
-Lemma irr_string : irreflexive string_ltb.
-Proof.
-move=>x; elim: x=>//=x xs.
-by move=>->; rewrite ascii_eqb_refl irr_ascii.
-Qed.
-
-(* Might be easier to define an embedding string -> seq ascii *)
-Lemma trans_string : transitive string_ltb.
-Proof. Admitted.
-
-Lemma total_string x y : [|| string_ltb x y, x == y | string_ltb y x].
-Proof. Admitted.
-
-Definition string_ordMixin := OrdMixin irr_string trans_string total_string.
-Canonical Structure string_ordType := Eval hnf in OrdType string string_ordMixin.
-
-End StringOrd.
-
-
-(** Instantiate the types *)
-Module TypesImpl <: Types.
-Definition Timestamp := N.
-Definition Hash := string.
-Definition VProof := unit.
-Definition Transaction := string.
-
-(* XXX Having to do this is immensely annoying. Is there a better way? *)
-Definition Hl (a b : Hash) := string_ltb a b.
-Lemma irr_Hl : irreflexive Hl. Proof. by apply irr_string. Qed.
-Lemma trans_Hl : transitive Hl. Proof. by apply trans_string. Qed.
-Lemma total_Hl x y : [|| Hl x y, x == y | Hl y x]. Proof. by apply total_string. Qed.
-
-Definition Hash_eqMixin := Eval hnf in EqMixin string_eqP.
-Canonical Hash_eqType := Eval hnf in EqType Hash Hash_eqMixin.
-Definition Hash_ordMixin := Eval hnf in OrdMixin irr_Hl trans_Hl total_Hl.
-Canonical Hash_ordType := Eval hnf in OrdType Hash Hash_ordMixin.
-
-Lemma VProof_eqP : Equality.axiom (fun _ _ : VProof => true). Proof. by case=>//=; case; constructor. Qed.
-Definition VProof_eqMixin := EqMixin VProof_eqP.
-Canonical VProof_eqType := Eval hnf in EqType VProof VProof_eqMixin.
-Definition ordtt (x y : VProof ) := false.
-Lemma irr_tt : irreflexive ordtt. Proof. by []. Qed.
-Lemma trans_tt : transitive ordtt. Proof. by []. Qed.
-Lemma total_tt x y : [|| ordtt x y, x == y | ordtt y x ]. Proof. by []. Qed.
-Definition VProof_ordMixin := OrdMixin irr_tt trans_tt total_tt.
-Canonical Structure VProof_ordType := Eval hnf in OrdType VProof VProof_ordMixin.
-
-Definition Tl (a b : Transaction) := string_ltb a b.
-Lemma irr_Tl : irreflexive Hl. Proof. by apply irr_string. Qed.
-Lemma trans_Tl : transitive Hl. Proof. by apply trans_string. Qed.
-Lemma total_Tl x y : [|| Tl x y, x == y | Tl y x]. Proof. by apply total_string. Qed.
-
-Definition Transaction_eqMixin := Eval hnf in EqMixin string_eqP.
-Canonical Transaction_eqType := Eval hnf in EqType Transaction Transaction_eqMixin.
-Definition Transaction_ordMixin := Eval hnf in OrdMixin irr_Tl trans_Tl total_Tl.
-Canonical Transaction_ordType := Eval hnf in OrdType Transaction Transaction_ordMixin.
-
-Record Block  :=
-  mkB {
-    prevBlockHash : Hash;
-    txs : seq Transaction;
-    proof : VProof;
-  }.
-
-Definition eq_block b b':=
-  match b, b' with
-  | mkB p t pf, mkB p' t' pf' =>
-    [&& p == p', t == t' & pf == pf']
-  end.
-
-Lemma eq_blockP : Equality.axiom eq_block.
-Proof.
-case=> p t pf; case=> p' t' pf'; rewrite /eq_block/=.
-case H2: (p == p'); [move/eqP: H2=>?; subst p'| constructor 2];
-  last by case=>?; subst p';rewrite eqxx in H2.
-case H3: (t == t'); [move/eqP: H3=>?; subst t'| constructor 2];
-  last by case=>?; subst t';rewrite eqxx in H3.
-case H4: (pf == pf'); [move/eqP: H4=>?; subst pf'| constructor 2];
-  last by case=>?; subst pf';rewrite eqxx in H4.
-by constructor 1.
-Qed.
-
-Canonical Block_eqMixin := Eval hnf in EqMixin eq_blockP.
-Canonical Block_eqType := Eval hnf in EqType Block Block_eqMixin.
-
-Definition block := Block.
-Definition Blockchain := seq block.
-
-Definition TxPool := seq Transaction.
-Definition BlockTree := union_map [ordType of Hash] block.
-End TypesImpl.
-
 (** Instantiate Toychain with a proof-of-work scheme **)
 Module ProofOfWork <: (ConsensusParams TypesImpl).
 Import TypesImpl.
 
 Definition GenesisBlock : block :=
-  mkB ((of_N 0) <: Hash) [::] (tt <: VProof).
+  mkB ((of_N 0) <: Hash)
+      [::]
+      (tt <: VProof).
 
 Definition subchain (bc1 bc2 : Blockchain) := exists p q, bc2 = p ++ bc1 ++ q.
 Definition bcLast (bc : Blockchain) := last GenesisBlock bc.
@@ -282,7 +54,8 @@ Definition FCR bc bc' : bool :=
 Notation "A > B" := (FCR A B).
 Notation "A >= B" := (A = B \/ A > B).
 
-Definition txValid (tx : Transaction) (bc : Blockchain) := true.
+Definition txValid (tx : Transaction) (bc : Blockchain) :=
+  tx \notin flatten (map (fun b => txs b) bc).
 
 (* bt is an argument to allow you to validate transactions before
     adding them to your pool. However, all transactions are valid for us.
@@ -294,7 +67,11 @@ Definition tpExtend (tp : TxPool) (bt : BlockTree) (tx : Transaction) :=
 (* You'd normally want some difficulty adjustment, but we're just toying around *)
 (* TODO: don't hardcode difficulty *)
 Definition VAF (b : Block) (bc : Blockchain) (tp : TxPool) : bool :=
-  if (16 <? (work b))%N then true else false.
+  (* GenesisBlock doesn't have work requirements *)
+  if (b == GenesisBlock) then
+    if (bc == [::]) && (tp == [::]) then true else false
+  (* All other blocks do *)
+  else if (16 <? (work b))%N then true else false.
 
 (* For proof-of-work, this would be more aptly called "getNonce" *)
 (* TODO: Implement this in the extraction *)
@@ -305,14 +82,16 @@ Parameter genProof : Blockchain -> TxPool -> Timestamp -> option (TxPool * VProo
 (*********************** <axioms> ***************************)
 (************************************************************)
 
-Axiom txValid_nil : forall t, txValid t [::].
+Lemma txValid_nil : forall t, txValid t [::].
+Proof. done. Qed.
 
 (** VAF **)
-Axiom VAF_init : VAF GenesisBlock [::] (txs GenesisBlock).
+Lemma VAF_init : VAF GenesisBlock [::] (txs GenesisBlock).
+Proof. by rewrite/VAF !eq_refl. Qed.
 
-Axiom VAF_GB_first :
+Lemma VAF_GB_first :
   forall bc, VAF GenesisBlock bc (txs GenesisBlock) -> bc = [::].
-
+Proof. by rewrite/VAF eq_refl=>bc; case: ifP=>//=; move/andP; case=>/eqP. Qed.
 
 (** FCR **)
 Axiom FCR_subchain :
