Extraction/Recipe.v
@@ -1,6 +1,6 @@
 Require Extraction.
 From Toychain
-Require Import Address Protocol Forests Parameters Impl.
+Require Import Address Protocol Forests Parameters TypesImpl Impl.
 Require Import ExtrOcamlBasic ExtrOcamlString ExtrOcamlZInt.
 
 (* Instantiate modules *)
@@ -17,11 +17,9 @@ Extraction Inline ssrbool.SimplPred.
 (* ordinals are nat, and we want to extract nat to int *)
 Extract Inductive nat => int [ "0" "succ" ] "(fun fO fS n -> if n=0 then fO () else fS (n-1))".
 
-Extract Constant ProofOfWork.hashT =>
-  "(fun tx -> ['0'; 'x'; '0'])".
+Extract Constant ProofOfWork.hashT => "Core.hash_of_tx".
 
-Extract Constant ProofOfWork.hashB =>
-  "(fun blk -> ['0'; 'x'; '0'])".
+Extract Constant ProofOfWork.hashB => "Core.hash_of_block".
 
 (* coq_Blockchain -> coq_TxPool -> coq_Timestamp -> *)
 (* (coq_TxPool * coq_VProof) option *)
